concurrency/machine_simulation.v
@@ -37,8 +37,9 @@ Variable init_inv : meminj -> G1 -> list val -> M1 -> G2 -> list val -> M2 -> Pr
 
 Variable halt_inv : (*SM_Injection*)meminj -> G1 -> val -> M1 -> G2 -> val -> M2 -> Prop.
 
-Variable runing_thread1 : C1 -> option nat.
-Variable runing_thread2 : C2 -> option nat.
+Variable tid: Type.
+Variable runing_thread1 : C1 -> option tid.
+Variable runing_thread2 : C2 -> option tid.
 
 Record Machine_sim  := 
 { core_data : Type
